50s great updateCurIndex

UnitProJ/expressOS/August/INode.dfy
@@ -22,7 +22,7 @@ if next == null then 1 else 1 + next.len()
 predicate good()
 reads this, footprint;
 {
-    this in footprint 
+    this in footprint && null !in footprint
 	&& (next != null ==> (next in footprint 
 	&& this !in next.footprint 
 	&& next.footprint + {this} == footprint
@@ -39,6 +39,9 @@ reads this, footprint;
 {
 good()  
 && (forall nd :: nd in spine ==> nd in footprint)
+&& listCond(spine)
+&& |spine| == |footprint|
+
 && (next != null ==> next.Valid())
 }
 
@@ -47,17 +50,14 @@ requires Valid();
 reads this, footprint;
 ensures ValidLemma();
 ensures |tailContents| == |footprint|-1 == |spine|-1;
-
-ensures forall nd :: nd in spine ==> nd != null && nd.Valid();
-
 ensures (forall i :: 1 <= i < |spine| ==> spine[i].data == tailContents[i-1]);
-//ensures ndSeq2DataSeq(spine) == [data] + tailContents;
+ensures ndSeq2DataSeq(spine) == [data] + tailContents;
 {
 (next == null) ||
 (next.ValidLemma())
 }
 
-
+/*
 constructor init(d:Data) 
 modifies this;
 ensures Valid();
@@ -94,15 +94,12 @@ r.spine := [r] + spine;
 return r;
 }
 
-/*
-method append(d:Data) returns (lastNd:INode)
+
+method append(d:Data)
 requires Valid();
 
 modifies footprint;
-//ensures Valid();
-//ensures fresh(lastNd);
-//ensures lastNd != null && lastNd.Valid();
-//ensures spine == old(spine) + [lastNd];
+ensures Valid();
 //ensures (tailContents == old(tailContents) + [d]);
 //ensures this.data == old(this.data);
 //ensures fresh(footprint - old(footprint));
@@ -125,49 +122,17 @@ tmpNd := tmpNd.next;
 index := index + 1;
 }
 
-
 tmpNd.next := node;
 
-ghost var mySeq := spine + [node];
+spine := spine + [node];
 
-
-
-/*
-assert mySeq[|mySeq|-2].footprint == {mySeq[|mySeq|-2]};
-
-assert listCond(mySeq[0..|mySeq|-1]);
-
-forall (nd | nd in spine)
-{
-nd.footprint := nd.footprint + {node};
-}
-
-assert listCond(mySeq[0..|mySeq|-1]);
-
-assert mySeq[|mySeq|-2].footprint == 
-{mySeq[|mySeq|-2]} + mySeq[|mySeq|-1].footprint;
-
-
-forall (nd | nd in spine)
-{
-nd.tailContents := nd.tailContents + [d];
-}
-
-assert listCond(mySeq[0..|mySeq|-1]);
-
-updateSeq(mySeq, |mySeq|-1);
-
-assert seqV(mySeq);
-
-assert spineFtprintLemma();
+updateSeq(spine, |spine|-1);
 assert ValidLemma();
-*/
 
-return node;
 
 }
-*/
 
+*/
 
 
 
@@ -201,7 +166,6 @@ else
 allV(myNode.next)
 }
 
-
 predicate seqV(mySeq: seq<INode>)
 requires listCond(mySeq);
 requires mySeq != [] ==> mySeq[0].Valid();
@@ -214,44 +178,22 @@ mySeq == [] || seqV(mySeq[1..])
 }
 
 
-predicate spineFtprintLemma()
+predicate ValidLemma2()
 requires Valid();
 reads this, footprint;
 
-ensures spineFtprintLemma();
+ensures ValidLemma2();
 ensures (set nd | nd in spine) == footprint;
+
+ensures forall nd :: nd in footprint ==> nd.footprint <= footprint;
 {
 if next == null then (spine == [this] && footprint == {this})
 else (
 spine == [this] + next.spine 
 && footprint == {this} + next.footprint
-&& next.spineFtprintLemma())
+&& next.ValidLemma2())
 }
 
-
-/*************************************/
-predicate ndValid2ListValidLemma()
-requires Valid();
-reads this, footprint;
-
-ensures ndValid2ListValidLemma();
-
-ensures forall nd :: nd in footprint ==> nd != null &&
-							nd.footprint <= footprint;
-
-ensures validSeqCond(spine);
-{
-if next == null then (spine == [this] && footprint == {this}
-					&& tailContents == [])
-else (
-this !in next.footprint &&
-spine == [this] + next.spine 
-&& footprint == {this} + next.footprint
-&& tailContents == [next.data] + next.tailContents
-&& next.ndValid2ListValidLemma())
-}
-
-}
 
 
 predicate allDiff(mySeq:seq<INode>)
@@ -274,119 +216,80 @@ if mySeq == [] then []
 else [mySeq[0].data] + ndSeq2DataSeq(mySeq[1..])
 }
 
-
-predicate listInv(mySeq: seq<INode>)
-reads mySeq, (set nd | nd in mySeq);
-{
-null !in mySeq && (forall nd :: nd in mySeq ==> nd in nd.footprint) &&
-(forall i :: 0 <= i < |mySeq|-1 ==> mySeq[i].next == mySeq[i+1])
-&& (forall i, j :: 0 <= i < j < |mySeq| ==> mySeq[i] !in mySeq[j].footprint)
-}
-
 predicate listCond(mySeq: seq<INode>)
 reads mySeq, (set nd | nd in mySeq);
 {
 null !in mySeq && (forall nd :: nd in mySeq ==> nd in nd.footprint) &&
-(forall i :: 0 <= i < |mySeq|-1 ==> mySeq[i].next == mySeq[i+1]
-	&& mySeq[i].footprint == {mySeq[i]} + mySeq[i+1].footprint
-	&& mySeq[i].tailContents == [mySeq[i+1].data] + mySeq[i+1].tailContents
-	&& mySeq[i].spine == [mySeq[i]] + mySeq[i+1].spine)
+allDiff(mySeq) &&
+(forall i :: 0 <= i < |mySeq|-1 ==> mySeq[i].next == mySeq[i+1])
 && (forall i, j :: 0 <= i < j < |mySeq| ==> mySeq[i] !in mySeq[j].footprint)
 }
 
+
+predicate goodSeqCond(mySeq: seq<INode>)
+reads mySeq, sumAllFtprint(mySeq);
+{
+listCond(mySeq) &&
+(forall nd :: nd in mySeq ==> nd.good())
+}
+
 predicate validSeqCond(mySeq: seq<INode>)
-reads mySeq, (set nd | nd in mySeq);
+reads mySeq, sumAllFtprint(mySeq);
 {
-listCond(mySeq) 
-&& (mySeq != [] ==> mySeq[|mySeq|-1].next == null
-&& mySeq[|mySeq|-1].footprint == {mySeq[|mySeq|-1]}
-&& mySeq[|mySeq|-1].tailContents == []
-&& mySeq[|mySeq|-1].spine == [mySeq[|mySeq|-1]])
+listCond(mySeq) &&
+(forall nd :: nd in mySeq ==> nd.Valid())
 }
 
-
-predicate validSeqLemma2(mySeq: seq<INode>)
-requires mySeq != [];
-
+//
+predicate validSeqLemma(mySeq:seq<INode>)
 requires validSeqCond(mySeq);
-reads mySeq, (set nd | nd in mySeq);
+requires mySeq != [] && mySeq[|mySeq|-1].next == null;
+reads mySeq, sumAllFtprint(mySeq);
+
+ensures mySeq[0].footprint == (set nd | nd in mySeq);
+{
+validSeqLemma2(mySeq) && mySeq[0].validSeqLemma3(mySeq)
+}
+
+predicate validSeqLemma2(mySeq:seq<INode>)
+requires validSeqCond(mySeq);
+requires mySeq != [] && mySeq[|mySeq|-1].next == null;
+reads mySeq, sumAllFtprint(mySeq);
 ensures validSeqLemma2(mySeq);
+
 ensures mySeq[0].spine == mySeq;
-ensures validSeqCond(mySeq[0].spine);
 {
-if |mySeq| == 1 then true
-else mySeq[0].spine == [mySeq[0]] + mySeq[1].spine
-	&& validSeqLemma2(mySeq[1..])
+mySeq[0].Valid() && (
+if |mySeq| == 1 then mySeq[0].next == null
+&& mySeq[0].spine == [mySeq[0]]
+else
+(mySeq[0].spine == [mySeq[0]] + mySeq[1].spine
+&& validSeqLemma2(mySeq[1..]))
+)
 }
 
-
-predicate validSeqFtprintInclusionLemma(mySeq: seq<INode>)
-requires mySeq != [];
-
-requires validSeqCond(mySeq);
-reads mySeq, (set nd | nd in mySeq);
-ensures validSeqFtprintInclusionLemma(mySeq);
-ensures forall nd :: nd in mySeq ==> nd in mySeq[0].footprint;
-{
-if |mySeq| == 1 then true
-else 
-	{mySeq[0]} + mySeq[1].footprint == mySeq[0].footprint &&
-	
-	validSeqFtprintInclusionLemma(mySeq[1..])
-}
-
-
-predicate validSeqGoodLemma(mySeq: seq<INode>)
-requires mySeq != [];
-
-requires validSeqCond(mySeq);
-reads mySeq, (set nd | nd in mySeq);
-ensures mySeq[0].good();
-{
-if |mySeq| == 1 then true
-else 
- mySeq[0].next == mySeq[1] &&
- mySeq[0] in mySeq[0].footprint &&
- mySeq[0] !in mySeq[1].footprint &&
- mySeq[1] in mySeq[0].footprint &&
- mySeq[0].spine == [mySeq[0]] + mySeq[1].spine &&
- mySeq[0].tailContents == [mySeq[1].data] + mySeq[1].tailContents
-}
-
-
-
-predicate validSeqLemma(mySeq: seq<INode>)
-requires mySeq != [];
-
-requires validSeqCond(mySeq);
-reads mySeq, (set nd | nd in mySeq);
-ensures validSeqLemma(mySeq);
-ensures mySeq[0].Valid();
-{
-if(|mySeq| == 1) then true
-else    
-	validSeqGoodLemma(mySeq) &&
-    validSeqLemma2(mySeq) &&
-    validSeqFtprintInclusionLemma(mySeq) &&
-    validSeqLemma(mySeq[1..])
-}
-
+predicate validSeqLemma3(mySeq:seq<INode>)
+requires Valid();
+requires spine == mySeq;
+reads this, footprint, mySeq;
+ensures (set nd | nd in spine) == footprint;
+ensures footprint == (set nd | nd in mySeq);
+{ValidLemma2()}
 
 //===============================================
 
-ghost method updateCurIndex(mySeq:seq<INode>, index:int, 
-				d:Data, newNd:INode)
-requires 0 <= index <= |mySeq| - 2;
-requires listInv(mySeq);
 
+ghost method updateCurIndex(mySeq:seq<INode>, index:int,
+			d:Data, newNd:INode)
+requires 0 <= index <= |mySeq| - 2;
+requires listCond(mySeq);
+requires mySeq[index+1].Valid();
+requires mySeq[index+1].spine == mySeq[index+1..];
+	
 requires forall i :: 0 <= i < index ==>
 	   mySeq[i].footprint == {mySeq[i]} + mySeq[i+1].footprint
 	&& mySeq[i].tailContents == [mySeq[i+1].data] + mySeq[i+1].tailContents
 	&& mySeq[i].spine == [mySeq[i]] + mySeq[i+1].spine;
-
-requires mySeq[index+1].spine == mySeq[index+1..];
-
-requires validSeqCond(mySeq[index+1..]);
 
 requires mySeq[index].footprint + {newNd} == 
 	{mySeq[index]} + mySeq[index+1].footprint;
@@ -397,18 +300,19 @@ requires mySeq[index].spine + [newNd] ==
 requires mySeq[index].tailContents + [d] == 
 	[mySeq[index+1].data] + mySeq[index+1].tailContents;
 
-modifies mySeq;
+modifies mySeq[index];
+//ensures fresh((set nd | nd in mySeq) - old(set nd | nd in mySeq));
 
-ensures listInv(mySeq);
+ensures listCond(mySeq);
 
-requires forall i :: 0 <= i < index-1 ==>
+ensures forall i :: 0 <= i < index-1 ==>
 	   mySeq[i].footprint == {mySeq[i]} + mySeq[i+1].footprint
 	&& mySeq[i].tailContents == [mySeq[i+1].data] + mySeq[i+1].tailContents
 	&& mySeq[i].spine == [mySeq[i]] + mySeq[i+1].spine;
 
-ensures mySeq[index].spine == mySeq[index..];
+ensures mySeq[index].Valid();
 
-ensures validSeqCond(mySeq[index..]);
+ensures mySeq[index].spine == mySeq[index..];
 
 ensures mySeq[index].footprint == old(mySeq[index].footprint) + {newNd};
 ensures mySeq[index].spine == old(mySeq[index].spine) + [newNd];
@@ -422,97 +326,48 @@ ensures index > 0 ==> (mySeq[index-1].footprint + {newNd} ==
 	mySeq[index-1].tailContents + [d] == 
 	[mySeq[index].data] + mySeq[index].tailContents);
 {
-mySeq[index].tailContents := mySeq[index].tailContents + [d];
+mySeq[index].tailContents := [mySeq[index+1].data] + mySeq[index+1].tailContents;
 
-mySeq[index].footprint := mySeq[index].footprint + {newNd};
+mySeq[index].footprint := {mySeq[index]} + mySeq[index+1].footprint;
 
-mySeq[index].spine := mySeq[index].spine + [newNd];
+mySeq[index].spine := [mySeq[index]] + mySeq[index+1].spine;
 }
 
 
-
-ghost method updateSeq(mySeq:seq<INode>, d:Data, newNd:INode)
-requires |mySeq| == 5;
-//requires |mySeq| > 1;
-requires listInv(mySeq);
-
-requires forall i :: 0 <= i < |mySeq|-2 ==>
-	   mySeq[i].footprint == {mySeq[i]} + mySeq[i+1].footprint
-	&& mySeq[i].tailContents == [mySeq[i+1].data] + mySeq[i+1].tailContents
-	&& mySeq[i].spine == [mySeq[i]] + mySeq[i+1].spine;
-
-
-requires mySeq[|mySeq|-1].spine == mySeq[|mySeq|-1..];
-requires validSeqCond(mySeq[|mySeq|-1..]);
-	
-requires mySeq[|mySeq|-2].footprint + {newNd} == 
-	{mySeq[|mySeq|-2]} + mySeq[|mySeq|-1].footprint;
-
-requires mySeq[|mySeq|-2].spine + [newNd] == 
-	[mySeq[|mySeq|-2]] + mySeq[|mySeq|-1].spine;
-
-requires mySeq[|mySeq|-2].tailContents + [d] == 
-	[mySeq[|mySeq|-1].data] + mySeq[|mySeq|-1].tailContents;
-
-
-modifies mySeq;
 /*
-ensures mySeq[0].footprint == old(mySeq[0].footprint) + {newNd};
-ensures mySeq[0].spine == old(mySeq[0].spine) + [newNd];
-ensures mySeq[0].tailContents == 
-	old(mySeq[0].tailContents) + [d];
+ghost method updateSeq(mySeq:seq<INode>, mid:int)
+
+requires mySeq != [];
+requires listCond(mySeq);
+
+requires 0 <= mid < |mySeq|;
+requires mySeq[mid].Valid();
+requires mySeq[mid].spine == mySeq[mid..];
+	
+modifies mySeq;
 
 ensures validSeqCond(mySeq);
-ensures mySeq[0].Valid();
-*/
+ensures fresh((set nd | nd in mySeq) - old(set nd | nd in mySeq));
 {
-
-ghost var index := |mySeq|-2;
+ghost var index := mid - 1;
 
 while(index >= 0)
-invariant -1 <= index <= |mySeq|-2;
-
-invariant listInv(mySeq);
-
-invariant forall i :: 0 <= i < |mySeq|-1 && i != index ==>
-	   mySeq[i].footprint == {mySeq[i]} + mySeq[i+1].footprint
-	&& mySeq[i].tailContents == [mySeq[i+1].data] + mySeq[i+1].tailContents
-	&& mySeq[i].spine == [mySeq[i]] + mySeq[i+1].spine;
-
+invariant -1 <= index <= mid - 1;
+invariant listCond(mySeq);
+invariant mySeq[index+1].Valid(); 
+invariant mySeq[mid].Valid();
 invariant mySeq[index+1].spine == mySeq[index+1..];
-
-invariant validSeqCond(mySeq[index+1..]);
-
-invariant index >= 0 ==> mySeq[index].footprint + {newNd} == 
-	{mySeq[index]} + mySeq[index+1].footprint;
-
-invariant index >= 0 ==> mySeq[index].spine + [newNd] == 
-	[mySeq[index]] + mySeq[index+1].spine;
-
-invariant index >= 0 ==> mySeq[index].tailContents + [d] == 
-	[mySeq[index+1].data] + mySeq[index+1].tailContents;
-
-
-invariant -1 <= index < |mySeq|-2 ==> (
- mySeq[index+1].footprint == old(mySeq[index+1].footprint) + {newNd} &&
- mySeq[index+1].spine == old(mySeq[index+1].spine) + [newNd] &&
- mySeq[index+1].tailContents == 
-	old(mySeq[index+1].tailContents) + [d]);
-
+invariant fresh((set nd | nd in mySeq) - old(set nd | nd in mySeq));
 {
-
-updateCurIndex(mySeq, index, d, newNd);
-//mySeq[index].tailContents := mySeq[index].tailContents + [d];
-
-//mySeq[index].footprint := mySeq[index].footprint + {newNd};
-
-//mySeq[index].spine := mySeq[index].spine + [newNd];
+updateCurIndex(mySeq, index);
 
 index := index - 1;
-
 }
 
-//assert validSeqLemma(mySeq);
+assert seqV(mySeq);
+}
+*/
+
+
 
 }
-
